\begin{align} &x_{eb}^{up} = {P_{eb}} + \sum\limits_{i = 1}^{{N_{eb}}} {\Delta P_{g,i}^{up}},x_{eb}^{dn} = {P_{eb\;{\rm{max}}}} - {P_{eb}} + \sum\limits_{g = 1}^{{N_{eb}}} {\Delta P_{g,i}^{dn}} \\ & {\text{s.t.}}\left\{ \begin{array}{l} \sum\nolimits_{i = 1}^{{N_{eb}}} {{\gamma _{g,i}}\Delta P_{g,i}^{up}} = {P_{eb}}{H_{eb\;{\rm{max}}}}/{P_{eb\;{\rm{max}}}}\\ \sum\nolimits_{i = 1}^{{N_{eb}}} {{\gamma _{g,i}}\Delta P_{g,i}^{dn}} = {H_{eb\;{\rm{max}}}} - {P_{eb}}{H_{eb\;{\rm{max}}}}/{P_{eb\;{\rm{max}}}} \end{array} \right. \end{align}
